feat: Finished Partial.dfy

examples/scalaEquivalenceBenchmarkExamples/Partial.dfy
@@ -3,9 +3,7 @@
 
 
 
-ghost function existsM<T(!new)>(p: T -> bool): bool
-  ensures existsM(p) <==> exists t: T :: p(t)
-{
+ghost function existsM<T(!new)>(p: T -> bool): bool {
   ! forall t: T :: !p(t)
 }
 
@@ -23,10 +21,7 @@ ghost function maxNegPM(j: int, p: int -> bool): bool {
 ghost function fM(x: int, p: int -> bool): int
   requires (!p(x) || existsM((j: int) => j < x && maxNegPM(j, p)))
   decreases(if (!p(x)) then 0 else x - eliminate_existsM((j: int) => j < x && maxNegPM(j, p))) {
-  if (p(x)) then 
-    var j :| j < x && !p(j) && forall k :: !p(k) ==> (k <= j);
-    assert j < x - 1 ==> exists j :: ((j: int) => j < x - 1 && maxNegPM(j, p))(j);
-    fM(x - 1, p)
+  if (p(x)) then termM(x, p); fM(x - 1, p)
   else x
   }
 
@@ -41,10 +36,31 @@ ghost function maxNegP(p: int -> bool, j: int): bool {
     forall k :: !p(k) ==> (k <= j)
 }
 
-function f(x: int, p: int -> bool): int
+lemma equiv(x: int, p: int -> bool) 
+  ensures existsM((j: int) => j < x && maxNegPM(j, p)) <==> existsF((j: int) => j < x && maxNegP(p, j))
+{
+  assert forall j: int :: !((j: int) => j < x && maxNegPM(j, p))(j) <==> !((j: int) => j < x && maxNegP(p, j))(j);
+}
+
+lemma termM(x: int, p: int -> bool)
+  requires (existsM((j: int) => j < x && maxNegPM(j, p)))
+  ensures (!p(x - 1) || existsM((j: int) => j < x - 1 && maxNegPM(j, p)))
+{
+  var j :| j < x && maxNegPM(j, p);
+  assert j < x - 1 ==> exists j :: ((j: int) => j < x - 1 && maxNegPM(j, p))(j);
+}
+
+lemma termF(x: int, p: int -> bool)
+  requires (existsF((j: int) => j < x && maxNegP(p, j)))
+  ensures (!p(x - 1) || existsF((j: int) => j < x - 1 && maxNegP(p, j)))
+{
+  equiv(x, p); termM(x, p); equiv(x - 1, p);
+}
+
+ghost function f(x: int, p: int -> bool): int
   requires (!p(x) || existsF((j: int) => j < x && maxNegP(p, j)))
-  decreases(if (!p(x)) then 0 else x - eliminate_existsM((j: int) => j < x && maxNegPM(j, p))) {
+  decreases(if (!p(x)) then 0 else equiv(x, p); x - eliminate_existsM((j: int) => j < x && maxNegPM(j, p))) {
   var t := p(x);
-  if t then f(x - 1, p)
+  if t then termF(x, p); f(x - 1, p)
   else x
   }
